theories/CombinatoryLogic/Plotkin.v
@@ -1,4 +1,6 @@
-(* plotkin call by value call by name and lambda calculus *)
+(*
+  [1] Plotkin, Gordon "Call-by-name, call-by-value and the λ-calculus." Theoretical computer science 1.2 (1975): 125-159.
+*)
 
 From Undecidability Require L.L.
 Require Import List Lia.
@@ -6,49 +8,11 @@ Import L.
 From Undecidability Require Import L.Util.L_facts.
 From Undecidability Require L.Computability.Seval.
 Require Import Relations.
+
+From Undecidability Require Import CombinatoryLogic.Krivine.
+
 Require Import ssreflect ssrbool ssrfun.
-
-Inductive eterm := closure : list eterm -> term -> eterm.
-
-(* actual krivine machine
-https://en.wikipedia.org/wiki/Krivine_machine *)
-Inductive halt_cbn : list eterm -> list eterm -> term -> Prop :=
-  | halt_var_0 ts ctx t ctx' :
-      halt_cbn ts ctx t ->
-      halt_cbn ts ((closure ctx t)::ctx') (var 0)
-  | halt_var_S ts ctx n t :
-      halt_cbn ts ctx (var n) ->
-      halt_cbn ts (t::ctx) (var (S n))
-  | halt_app ts ctx s t :
-      halt_cbn ((closure ctx t)::ts) ctx s ->
-      halt_cbn ts ctx (app s t)
-  | halt_lam_ts t ts ctx s :
-      halt_cbn ts (t::ctx) s ->
-      halt_cbn (t::ts) ctx (lam s)
-  | halt_lam ctx s :
-      halt_cbn [] ctx (lam s).
-
-Lemma halt_cbnE ts ctx u : halt_cbn ts ctx u ->
-  match u with
-  | var 0 =>
-      match ctx with
-      | [] => False
-      | (closure ctx' t')::_ => halt_cbn ts ctx' t'
-      end
-  | var (S n) => 
-      match ctx with
-      | [] => False
-      | _::ctx' => halt_cbn ts ctx' (var n)
-      end
-  | app s t => halt_cbn ((closure ctx t) :: ts) ctx s
-  | lam s =>
-      match ts with
-      | [] => True
-      | t'::ts' => halt_cbn ts' (t'::ctx) s
-      end
-  end.
-Proof. by case. Qed.
-    
+   
 (* left-most outer-most call-by-name *)
 Inductive step : term -> term -> Prop :=
   | stepLam s t    : step (app (lam s) t) (subst s 0 t)
@@ -72,7 +36,7 @@ Fixpoint ren (xi : nat -> nat) (t : term) : term  :=
 Fixpoint cbv_cbn (t : term) : term :=
   match t with
   | var n => lam (app (var 0) (var (S n)))
-  | app s t => lam (app (ren S (cbv_cbn  s)) (lam (app (ren S (ren S (cbv_cbn t))) (lam (app (app (var 1) (var 0)) (var 2))))))
+  | app s t => lam (app (ren S (cbv_cbn s)) (lam (app (ren S (ren S (cbv_cbn t))) (lam (app (app (var 1) (var 0)) (var 2))))))
   | lam s => lam (app (var 0) (ren S (lam (cbv_cbn s))))
   end.
 
@@ -86,7 +50,7 @@ Definition Psi (t : term) :=
 Lemma subst_ren s k t : subst (ren S s) (S k) t = ren S (subst s k t).
 Proof. Admitted. (* needs closedness *)
 
-Lemma subst_main M N k : 
+Lemma lemma_6_1 M N k : 
   subst (cbv_cbn M) k (Psi (lam N)) = cbv_cbn (subst M k (lam N)).
 Proof.
   elim: M k N.
@@ -102,9 +66,38 @@ Proof.
     cbn.
 Admitted.
 
-    done.
-    + done.
-    + done. cbn. done. 
+Definition on_app {X : Type} (s : term) (x : X) (g : term -> term -> X) : X :=
+  match s with
+  | app s t => g s t
+  | _ => x
+  end.
+
+(* plotkins M : K *)
+Fixpoint colon (M : term) (u : term) : term :=
+  on_app M (
+    app u (Psi M)
+  ) (
+    fun s t =>
+      on_app s (
+        on_app t (
+          app (app (Psi s) (Psi t)) u
+        ) (
+          fun t1 t2 => app (Psi t) (lam (app (app (app (var 0) (Psi s)) (var 0)) u))
+        )
+      ) (
+        fun s1 s2 => colon s (lam (app (cbv_cbn t) (lam (app (app (var 1) (var 0)) u))))
+      )
+  ).
+
+
+Lemma lemma_6_2 s u : closed (lam u) -> halt_cbn [] [] (colon s u) -> halt_cbn [] [] (app (cbv_cbn s) u).
+Proof.
+  move=> Hu. elim: s.
+  - move=> n /=.
+    move=> /halt_cbnE H'.
+    do ? constructor.
+    apply: (halt_cbn_flatten_iff H').
+
 
 Lemma main s t : s ≻ t -> 
   halt_cbn [] [] (app (cbv_cbn s) (lam (var 0))) -> 
