theories/CombinatoryLogic/Krivine.v
@@ -1,0 +1,187 @@
+(*
+  Krivine Machine
+  https://en.wikipedia.org/wiki/Krivine_machine
+
+  Closure-based left-most-outer-most lambda-term evaluation
+
+  Further details in L_CBN_Interpreter
+*)
+
+From Undecidability Require L.L.
+Require Import List Lia.
+Import L.
+From Undecidability Require Import L.Util.L_facts.
+From Undecidability Require L.Computability.Seval.
+Require Import Relations.
+Require Import ssreflect ssrbool ssrfun.
+
+Unset Implicit Arguments.
+
+Inductive eterm := closure : list eterm -> term -> eterm.
+
+(* actual krivine machine
+https://en.wikipedia.org/wiki/Krivine_machine *)
+Inductive halt_cbn : list eterm -> list eterm -> term -> Prop :=
+  | halt_var_0 ts ctx t ctx' :
+      halt_cbn ts ctx t ->
+      halt_cbn ts ((closure ctx t)::ctx') (var 0)
+  | halt_var_S ts ctx n t :
+      halt_cbn ts ctx (var n) ->
+      halt_cbn ts (t::ctx) (var (S n))
+  | halt_app ts ctx s t :
+      halt_cbn ((closure ctx t)::ts) ctx s ->
+      halt_cbn ts ctx (app s t)
+  | halt_lam_ts t ts ctx s :
+      halt_cbn ts (t::ctx) s ->
+      halt_cbn (t::ts) ctx (lam s)
+  | halt_lam ctx s :
+      halt_cbn [] ctx (lam s).
+
+Lemma halt_cbnE ts ctx u : halt_cbn ts ctx u ->
+  match u with
+  | var 0 =>
+      match ctx with
+      | [] => False
+      | (closure ctx' t')::_ => halt_cbn ts ctx' t'
+      end
+  | var (S n) => 
+      match ctx with
+      | [] => False
+      | _::ctx' => halt_cbn ts ctx' (var n)
+      end
+  | app s t => halt_cbn ((closure ctx t) :: ts) ctx s
+  | lam s =>
+      match ts with
+      | [] => True
+      | t'::ts' => halt_cbn ts' (t'::ctx) s
+      end
+  end.
+Proof. by case. Qed.
+
+Fixpoint term_size (t : term) : nat :=
+  match t with
+  | var n => n
+  | app s t => 1 + term_size s + term_size t
+  | lam s => 1 + term_size s
+  end.
+
+Fixpoint eterm_size (u : eterm) : nat :=
+  let '(closure ctx t) := u in 1 + list_sum (map eterm_size ctx) + (term_size t).
+
+Definition context_size (ctx : list eterm) : nat :=
+  eterm_size (closure ctx (var 0)).
+
+Fixpoint eclosed (u : eterm) : Prop :=
+  let '(closure ctx t) := u in bound (length ctx) t /\ Forall id (map eclosed ctx).
+
+Fixpoint subst_list k (ts : list term) (u : term) : term :=
+  match u with
+  | var n => nth n ((map var (seq 0 k)) ++ ts) (var n)
+  | app s t => app (subst_list k ts s) (subst_list k ts t)
+  | lam s => lam (subst_list (S k) ts s)
+  end.
+
+(* recursively substitute each local context *)
+Fixpoint flatten (u : eterm) : term :=
+  let '(closure ctx t) := u in subst_list 0 (map flatten ctx) t.
+
+  
+(* induction/recursion principle wrt. a decreasing measure f *)
+(* example: elim /(measure_rect length) : l. *)
+Lemma measure_rect {X : Type} (f : X -> nat) (P : X -> Type) : 
+(forall x, (forall y, f y < f x -> P y) -> P x) -> forall (x : X), P x.
+Proof.
+exact: (well_founded_induction_type (Wf_nat.well_founded_lt_compat X f _ (fun _ _ => id)) P).
+Qed.
+
+Lemma flatten_var_S t ctx n :
+  flatten (closure (t :: ctx) (var (S n))) = flatten (closure ctx (var n)).
+Proof.
+Admitted.
+
+Lemma Forall2_consE {X : Type} {P : X -> X -> Prop} {x1 l1 x2 l2} : 
+  Forall2 P (x1::l1) (x2::l2) -> P x1 x2 /\ Forall2 P l1 l2.
+Proof. move=> H. by inversion H. Qed.
+
+(* halt_cbn is invariant closure flattening *)
+Lemma halt_cbn_flatten_iff ts1 ts2 ctx1 ctx2 s1 s2:
+  halt_cbn ts1 ctx1 s1 ->
+  Forall2 (fun t1 t2 => flatten t1 = flatten t2) ts1 ts2 ->
+  flatten (closure ctx1 s1) = flatten (closure ctx2 s2) ->
+  halt_cbn ts2 ctx2 s2.
+Proof.
+  move=> H. elim: H ts2 ctx2 s2; clear ts1 ctx1 s1.
+  - move=> ts ctx t ctx' ? IH ts2 ctx2 s2.
+    by move=> /IH /[apply].
+  - move=> ts1 ctx1 n t ? IH ts2 ctx2 s2.
+    rewrite flatten_var_S.
+    by move=> /IH /[apply].
+  - move=> ts1 ctx1 s t ? IH ts2 ctx2 s2.
+    elim /(measure_rect context_size): ctx2 s2.
+    move=> ctx2 IH' []. 
+    + (* s2 is (var n) *)
+      move: ctx2 IH' => [|[ctx'2 t'2] ctx2] IH'. { by case. }
+      move=> [|n].
+      * move=> /= ??. apply: halt_var_0. apply: IH' => //=.
+        rewrite /context_size /=. lia.
+      * rewrite flatten_var_S.
+        move=> /= ??. apply: halt_var_S. apply: IH' => //=.
+        rewrite /context_size /=. lia.
+    + move=> ??? /= [] /IH {}IH ?.
+      apply: halt_app. apply: IH => //=.
+      by constructor.
+    + done.
+  - move=> t1 ts1 ctx1 s1 ? IH [|t2 ts2] ctx2 s2.
+    { move=> H. by inversion H. }
+    move=> /Forall2_consE [Ht1t2 ?].
+    elim /(measure_rect context_size): ctx2 s2.
+    move=> ctx2 IH' []. 
+    + (* s2 is (var n) *)
+      move: ctx2 IH' => [|[ctx'2 t'2] ctx2] IH'. { by case. }
+      move=> [|n].
+      * move=> /= ?. apply: halt_var_0. apply: IH'=> //=.
+        rewrite /context_size /=. lia.
+      * rewrite flatten_var_S.
+        move=> /= ?. apply: halt_var_S. apply: IH' => //=.
+        rewrite /context_size /=. lia.
+    + done.
+    + (* may still work with proper flatten (subst with shift, no var 0 as target because of shift) *) move=> ? [] /= ?.
+      apply: halt_lam_ts. apply: IH => //=.
+      rewrite Ht1t2.
+      subst_list 1 (var 0) (var 1) =
+      var 0 =
+      subst_list 1 (var 0) (var 0)
+
+      subst_list 0 (x :: (var 0)) (var 1)
+      = var 0 <> x =
+      subst_list 0 (x :: (var 0)) (var 0)
+      admit. (* doublecheck, here is closedness! *)
+  - move=> ctx1 s1 [|t2 ts2] ctx2 s2; first last.
+    { move=> H. by inversion H. }
+    move=> _.
+    elim /(measure_rect context_size): ctx2 s2.
+    move=> ctx2 IH' []. 
+    + (* s2 is (var n) *)
+      move: ctx2 IH' => [|[ctx'2 t'2] ctx2] IH'. { by case. }
+      move=> [|n].
+      * move=> /= ?. apply: halt_var_0. apply: IH'=> //=.
+        rewrite /context_size /=. lia.
+      * rewrite flatten_var_S.
+        move=> /= ?. apply: halt_var_S. apply: IH' => //=.
+        rewrite /context_size /=. lia.
+    + done.
+    + move=> *. by apply: halt_lam.
+
+
+(* halt_cbn is invariant closure flattening *)
+Lemma halt_cbn_flatten_iff ts1 ts2 ctx1 ctx2 s1 s2:
+  halt_cbn ts1 ctx1 s1 ->
+  Forall id (map eclosed ts1) ->
+  Forall id (map eclosed ts2) ->
+  Forall2 (fun t1 t2 => flatten t1 = flatten t2) ts1 ts2 ->
+  eclosed (closure ctx1 s1) ->
+  eclosed (closure ctx2 s2) ->
+  flatten (closure ctx1 s1) = flatten (closure ctx2 s2) ->
+  halt_cbn ts2 ctx2 s2.
+Proof.
+Admitted.
